src/HOL/Number_Theory/MiscAlgebra.thy
@@ -155,12 +155,12 @@ lemma (in comm_group) power_order_eq_one:
     and a [simp]: "a : carrier G"
   shows "a (^) card(carrier G) = one G"
 proof -
-  have "(\<Otimes>x:carrier G. x) = (\<Otimes>x:carrier G. a \<otimes> x)"
+  have "(\<Otimes>x\<in>carrier G. x) = (\<Otimes>x\<in>carrier G. a \<otimes> x)"
     by (subst (2) finprod_reindex [symmetric],
       auto simp add: Pi_def inj_on_const_mult surj_const_mult)
-  also have "\<dots> = (\<Otimes>x:carrier G. a) \<otimes> (\<Otimes>x:carrier G. x)"
+  also have "\<dots> = (\<Otimes>x\<in>carrier G. a) \<otimes> (\<Otimes>x\<in>carrier G. x)"
     by (auto simp add: finprod_multf Pi_def)
-  also have "(\<Otimes>x:carrier G. a) = a (^) card(carrier G)"
+  also have "(\<Otimes>x\<in>carrier G. a) = a (^) card(carrier G)"
     by (auto simp add: finprod_const)
   finally show ?thesis
 (* uses the preceeding lemma *)
